Working on the reversal example. Encountered a weird problem apply induction.

Ann_Com.thy
@@ -8,16 +8,20 @@ type_synonym newstate = "address \<Rightarrow> int"
 type_synonym assn = "newstate \<Rightarrow> bool"
 
 datatype com =
-  Basic "newstate \<Rightarrow> newstate"      |
+  Basic "newstate \<Rightarrow> newstate"   ("BASIC _ ")   |
   Seq   com com          ("_;; _") |
   Cond "newstate \<Rightarrow> bool" com com      ("IF _ THEN _ ELSE _ FI")|
   While "newstate \<Rightarrow> bool" assn com    ("WHILE _ INV _ DO _ OD")|
   Wait "newstate \<Rightarrow> bool"              ("WAIT _ END")
 
 fun list :: "newstate \<Rightarrow> (int list) \<Rightarrow> int \<Rightarrow> bool" where 
-"list s [] i = (i = 0)"|
-"list s (x#xs) i = (\<exists>j. (s i = x) \<and> (s (i + 1) = j) \<and> list s xs j)"
+"list s [] i = (i = (0::int))"|
+"list s (x#xs) i = (\<exists>j. (s i = j) \<and> (s (i+1) = x) \<and> list s xs j)"
 
+(* s where "s \<equiv> \<lambda> i . if i = 1 then 3 else (if i = 2 then 42 else (if i = 3 then 0 else 43))"
+
+lemma "list s [42, 43] 1" by force
+*)
 fun reach_step::"newstate \<Rightarrow> nat \<Rightarrow> int \<Rightarrow> int \<Rightarrow> bool" where
 "reach_step s 0 i j = (i = j)"|
 "reach_step s (Suc n) i j = (\<exists>a k. (s i = a) \<and> (s (i + 1) = k) \<and> (reach_step s n k j))"
@@ -26,7 +30,7 @@ definition reach::"newstate \<Rightarrow> int \<Rightarrow> int \<Rightarrow> bo
   "reach s i j \<equiv> (\<exists>n \<ge> 0. reach_step s n i j)"
 
 datatype acom =
-  ABasic assn "newstate \<Rightarrow> newstate"      |
+  ABasic assn "newstate \<Rightarrow> newstate"    ("{_} BASIC _ ")   |
   ASeq   acom acom   ("_;; _") |
   ACond assn "newstate \<Rightarrow> bool" acom acom     ("{_} IF _ THEN _ ELSE _ FI")|
   AWhile assn "newstate \<Rightarrow> bool" assn acom    ("{_} WHILE _ INV _ DO _ OD")|
