Reversal.thy
@@ -2,6 +2,18 @@ theory Reversal
 imports VCG
 begin
 
+locale list_rev_example =
+fixes i::int and j::int and k::int
+begin
+
+abbreviation list_rev where
+"list_rev \<equiv> 
+  BASIC (\<lambda> s . s(j := 0));;
+  WHILE (\<lambda> s . s i \<noteq> 0) 
+    INV (\<lambda> s . True)
+    DO BASIC (\<lambda>s. s(k := s (i + 1), s (i + 1) := j, j := i, i := k))
+    OD"
+
 abbreviation pre0::"assn" where "pre0 \<equiv> \<lambda>s. \<exists>\<alpha> \<beta>. (list s \<alpha> i) \<and> (list s \<beta> j) \<and> (rev \<alpha> = (append (rev \<alpha>) \<beta>))"
 
 abbreviation loopcom::"newstate \<Rightarrow> newstate" where 
@@ -9,6 +21,5 @@ abbreviation loopcom::"newstate \<Rightarrow> newstate" where
 
 abbreviation revers::
 
-abbreviation 
-
+end
 end
